Refactor `byte` => `UInt8`
This also refactors a few other similar things.  For example, `u4`
becomes `UInt4` and `u256` because `UInt256` to keep the naming
consistent.

src/Main.lean
@@ -6,3 +6,12 @@ import LeanEVM.State
 
 def main : IO Unit :=
   IO.println "Hello world"
+
+
+abbrev byte2 := Fin 256
+
+def test(n:List byte2) := n.length
+
+example : (test [1,2]) = 2 :=
+by
+  simp_arith
