src/LeanEVM/Util/Lemmas.lean
@@ -7,8 +7,8 @@ by
   exact Nat.mul_le_mul_left m p
 
 -- A simple proof for "left shifting" bytes.  This could no doubt be generalised.
-def pow256_shift(n:Nat)(m:Fin 256)(k:Nat)(p:n < 256^k) : (256*n + m.val < 256^(k+1)) :=
+def pow256_shift(n:Nat)(m:UInt8)(k:Nat)(p:n < 256^k) : (256*n + m.val < 256^(k+1)) :=
 by
   have s : 256*n + 256 ≤ 256^(k+1) := (pow_shift n 256 k p)
-  have r : 256*n + m.val < 256*n + 256 := by exact Fin.natAdd.proof_1 (256 * n) m
+  have r : 256*n + m.val < 256*n + 256 := by exact Fin.natAdd.proof_1 (256 * n) m.val
   exact Nat.lt_of_lt_of_le r s
